Redo BST preservation

TreeTraversals.v
@@ -39,10 +39,125 @@ end.
 Fixpoint insert (n : nat) (t : BST) : BST := match t with
 | Leaf => Node Leaf n Leaf
 | Node l v r =>
-    if Nat.eqb n v then Node l v r else
-    if Nat.ltb n v then Node (insert n l) v r else
-    Node l v (insert n r)
+    if Nat.eqb n v then Node l v r
+    else
+        if Nat.ltb n v then Node (insert n l) v r
+        else Node l v (insert n r)
 end.
+
+(* Verifies that at BST is ordered *)
+Fixpoint isBST (t : BST) : bool := match t with
+| Leaf => true (* Vacuously tree*)
+| Node l v r =>
+    andb (andb (isBST l) (isBST r))
+    (match l with
+    | Leaf => match r with
+        | Leaf => true (* Value with two leaf children *)
+        | Node _ vr _ => Nat.ltb v vr (* One leaf, one child *)
+        end
+    | Node _ vl _ => andb (Nat.ltb vl v) (match r with
+        | Leaf => true (* One child, one leaf*)
+        | Node _ vr _ => (Nat.ltb v vr) (* Two children *)
+        end)
+    end)
+end.
+
+Lemma true_eq_true_imp_A : forall {A : Prop}, (true = true -> A) <-> A.
+Proof.
+  split.
+  - intros H. apply H. reflexivity.
+  - intros H _. exact H.
+Qed.
+
+Lemma insert_order : forall (t : BST) (n : nat), isBST t -> match insert n t 
+
+(* Show that insertion does not change a BST's status *)
+
+Lemma insert_preserves_BST (t : BST) (n : nat) :
+    isBST t = true -> isBST (insert n t) = true.
+Proof.
+    (*  l is the left subtree.
+        IHtl is its IH. v is the value.
+        r is the right subtree.
+        IHtr is its IH.
+    *)
+    induction t as [| l IHtl v r IHtr].
+    (* Insert into Leaf. *)
+    - simpl. reflexivity.
+
+    (* Insert into Node(l, v, r). *)
+    - intros. simpl. case_eq (Nat.eqb n v); intros H_v_eq_v.
+        + exact H.
+        + (* First tactic – show that left and right are balanced *)
+            assert (H' := H). apply andb_true_iff in H. destruct H as [Hsubtrees _].
+            apply andb_true_iff in Hsubtrees.  destruct Hsubtrees as [Hl Hr].
+            fold isBST in Hl. fold isBST in Hr.
+        
+            case_eq (Nat.ltb n v) ; intros H_v_lt_v.
+                * simpl. apply andb_true_iff. split.
+                {
+                    (* Left subtree preserves post insertion. *)
+                    apply andb_true_iff. split. {
+                        assert (IHtl_handy := IHtl). rewrite Hl in IHtl_handy. rewrite true_eq_true_imp_A in IHtl_handy. exact IHtl_handy.
+                    }
+                    (* Right subtree preserves. *)
+                    exact Hr.
+                }
+                { case_eq (insert n l); intros H_insl_leaf.
+                    (* Prove that right side is fine *)
+                    - destruct r as [| rl rv rr].
+                        + reflexivity.
+                        + intros. unfold isBST in H'. apply andb_true_iff in H'.
+                            destruct H' as [_ Hrec]. case_eq l; intros.
+                            * rewrite H in Hrec. exact Hrec.
+                            * rewrite H in Hrec. apply andb_true_iff in Hrec. destruct Hrec. exact H1. 
+                    - (* Prove that left side is fine *)
+                        intros. apply andb_true_iff. split.
+                        (* Left side fine *)
+                        + rewrite H in IHtl. apply IHtl in Hl. case_eq (Nat.leb n n0); intros H_n_le_n0.
+                            * admit.
+                            * apply Nat.ltb_lt in  H_v_lt_v. apply Nat.leb_nle in  H_n_le_n0.
+                            apply Nat.nle_gt in H_n_le_n0. 
+                            apply (Nat.lt_trans n0 n v) in H_n_le_n0. apply Nat.ltb_lt. exact H_n_le_n0. exact H_v_lt_v.
+                        (* Rights side fine *)
+                        + destruct r.
+                            * reflexivity.
+                            * unfold isBST in H'. apply andb_true_iff in H'.
+                            destruct H' as [_ Hrec]. case_eq l; intros.
+                                { 
+                                    rewrite H0 in Hrec. exact Hrec.
+                                }
+                                {
+                                    rewrite H0 in Hrec. apply andb_true_iff in Hrec.
+                                    destruct Hrec. exact H2.
+                                }
+                }
+
+                * simpl. apply andb_true_iff. split.
+                {   
+                    (* Left subtree preserves. *)
+                    apply andb_true_iff. split. exact Hl. 
+                    (* Right subtree preserves post insertion. *)
+                    assert (IHtr_handy := IHtr). rewrite Hr in IHtr_handy. rewrite true_eq_true_imp_A in IHtr_handy. exact IHtr_handy.
+                }
+                {  case_eq (insert n r); intros H_insr_leaf.
+                    (* Prove that left side is fine *)
+                    - destruct l as [| ll lv lr].
+                        + reflexivity.
+                        + intros. unfold isBST in H'. apply andb_true_iff in H'.
+                        destruct H' as [_ Hrec]. case_eq r; intros.
+                            * rewrite H in Hrec. exact Hrec.
+                            * apply andb_true_iff. split.
+                                {
+                                    rewrite H in Hrec. apply andb_true_iff in Hrec. destruct Hrec. exact H0.
+                                }
+                                {
+                                    reflexivity.
+                                }
+                    - (* Prove that right side is fine *)
+                        admit.
+                }
+Admitted. 
 
 (* Inorder traversal of a BST *)
 Fixpoint inorder (t : BST) : list nat := match t with
